Began work on region composition primitives

DeBruijnSSA/BinSyntax/Syntax/Compose/Region.lean
@@ -1,3 +1,169 @@
 import DeBruijnSSA.BinSyntax.Syntax.Subst
 
 namespace BinSyntax
+
+namespace Region
+
+def lsubst0 (r : Region φ) : Subst φ
+  | 0 => r
+  | ℓ + 1 => br ℓ (Term.var 0)
+
+def alpha (ℓ : ℕ) (r : Region φ) : Subst φ
+  := Function.update Subst.id ℓ r
+
+def ret (e : Term φ) := br 0 e
+
+def nil : Region φ := ret (Term.var 0)
+
+@[simp]
+def alpha0_nil : alpha 0 nil = @Subst.id φ := by
+  rw [alpha, Function.update_eq_self_iff]
+  rfl
+
+def append (r r' : Region φ) : Region φ := r.lsubst (r'.alpha 0).vlift
+
+instance : Append (Region φ) := ⟨Region.append⟩
+
+theorem append_def (r r' : Region φ) : r ++ r' = r.lsubst (r'.alpha 0).vlift := rfl
+
+@[simp]
+theorem append_nil (r : Region φ) : r ++ nil = r := by simp [append_def]
+
+@[simp]
+theorem nil_append (r : Region φ) : nil ++ r = r := by
+  simp only [append_def, lsubst, Subst.vlift, alpha, Function.comp_apply, Function.update_same]
+  rw [<-vsubst_fromWk_apply, <-vsubst_comp_apply, <-vsubst_id r]
+  congr <;> simp
+
+-- TODO: ret append ret should be alpha0 or smt...
+
+@[simp]
+theorem Subst.vwk_liftWk_comp_id : vwk (Nat.liftWk ρ) ∘ id = @id φ := rfl
+
+@[simp]
+theorem Subst.vwk_liftnWk_comp_id (n : ℕ) : vwk (Nat.liftnWk (n + 1) ρ) ∘ id = @id φ := by
+  rw [Nat.liftnWk_succ']
+  rfl
+
+theorem append_assoc (r r' r'' : Region φ) : (r ++ r') ++ r'' = r ++ (r' ++ r'')
+  := by
+  simp only [append_def, lsubst_lsubst]
+  congr
+  funext ℓ
+  simp only [
+    Subst.comp, Subst.vlift, alpha, Function.comp_apply, Function.comp_update,
+    Subst.vwk_liftWk_comp_id, vwk_vwk
+  ]
+  cases ℓ with
+  | zero =>
+    simp only [
+      Function.update_same, vwk_lsubst, Function.comp_update, Subst.vwk_liftWk_comp_id, vwk_vwk]
+    apply congrFun
+    apply congrArg
+    apply congrArg
+    congr
+    funext n
+    cases n <;> rfl
+  | succ => rfl
+
+def Subst.left_label_distrib (e : Term φ) : Subst φ
+  := λℓ => br ℓ (Term.pair (e.wk Nat.succ) (Term.var 0))
+
+def Subst.right_label_distrib (e : Term φ) : Subst φ
+  := λℓ => br ℓ (Term.pair (Term.var 0) (e.wk Nat.succ))
+
+def left_label_distrib (r : Region φ) (e : Term φ) : Region φ
+  := r.lsubst (Subst.left_label_distrib e)
+
+def right_label_distrib (r : Region φ) (e : Term φ) : Region φ
+  := r.lsubst (Subst.right_label_distrib e)
+
+def left_distrib (r : Region φ) : Region φ
+  := ((r.vwk Nat.succ).left_label_distrib (Term.var 0)).let2 (Term.var 0)
+
+def right_distrib (r : Region φ) : Region φ
+  := ((r.vwk (Nat.liftWk Nat.succ)).right_label_distrib (Term.var 1)).let2 (Term.var 0)
+
+-- TODO: label threading vs. distribution, equal if fvi ≤ 1
+
+def associator : Region φ :=
+  let2 (Term.var 0) $
+  let2 (Term.var 0) $
+  ret (Term.pair (Term.var 0) (Term.pair (Term.var 1) (Term.var 2)))
+
+def associator_inv : Region φ :=
+  let2 (Term.var 0) $
+  let2 (Term.var 1) $
+  ret (Term.pair (Term.pair (Term.var 2) (Term.var 0)) (Term.var 1))
+
+def proj_left : Region φ :=
+  let2 (Term.var 0) $
+  ret (Term.var 0)
+
+def proj_right : Region φ :=
+  let2 (Term.var 0) $
+  ret (Term.var 1)
+
+def left_unitor_inv : Region φ := ret (Term.pair Term.unit (Term.var 0))
+
+def right_unitor_inv : Region φ := ret (Term.pair (Term.var 0) Term.unit)
+
+def inl : Region φ := ret (Term.var 0).inl
+
+def inr : Region φ := ret (Term.var 0).inr
+
+def swap : Region φ :=
+  let2 (Term.var 0) $
+  ret (Term.pair (Term.var 1) (Term.var 0))
+
+def let_eta : Region φ :=
+  let1 (Term.var 0) $
+  ret (Term.var 0)
+
+def let2_eta : Region φ :=
+  let2 (Term.var 0) $
+  ret (Term.pair (Term.var 0) (Term.var 1))
+
+def case_eta : Region φ := case (Term.var 0) (ret (Term.var 0)) (ret (Term.var 0))
+
+def drop : Region φ :=
+  let1 (Term.var 0) $
+  ret Term.unit
+
+def join (r r' : Region φ) : Region φ := case (Term.var 0)
+  (r.vwk (Nat.liftWk Nat.succ))
+  (r'.lwk (Nat.liftWk Nat.succ))
+
+def abort : Region φ := ret (Term.var 0).abort
+
+def left_distributor : Region φ :=
+  let2 (Term.var 0) $
+  case (Term.var 1)
+    (ret (Term.pair (Term.var 0) (Term.var 1)))
+    (ret (Term.pair (Term.var 0) (Term.var 1)))
+
+def right_distributor : Region φ :=
+  let2 (Term.var 0) $
+  case (Term.var 0)
+    (ret (Term.pair (Term.var 2) (Term.var 0)))
+    (ret (Term.pair (Term.var 2) (Term.var 0)))
+
+def right_exit : Region φ :=
+  case (Term.var 0)
+    (br 0 (Term.var 0))
+    (br 1 (Term.var 0))
+
+def left_exit : Region φ :=
+  case (Term.var 0)
+    (br 1 (Term.var 0))
+    (br 0 (Term.var 0))
+
+def fixpoint (r : Region φ) : Region φ := cfg nil 1 (λ_ => r ++ left_exit)
+
+def ite (b : Term φ) (r r' : Region φ) : Region φ := case b (r.vwk Nat.succ) (r'.vwk Nat.succ)
+
+def wappend (r r' : Region φ) : Region φ := cfg r 1 (λ_ => r'.lwk Nat.succ)
+
+end Region
+
+end BinSyntax
