DeBruijnSSA/BinSyntax/Syntax/Fv/Subst.lean
@@ -11,7 +11,31 @@ namespace BinSyntax
 /-! ### Lemmas about substitution -/
 section Subst
 
+@[simp]
 theorem Terminator.fl_vsubst (σ : Term.Subst φ) (r : Terminator φ) : (r.vsubst σ).fl = r.fl := by
   induction r generalizing σ <;> simp [*]
+
+@[simp]
+theorem TRegion.fl_vsubst (σ : Term.Subst φ) (r : TRegion φ) : (r.vsubst σ).fl = r.fl := by
+  induction r generalizing σ <;> simp [*]
+
+@[simp]
+theorem Block.fl_vsubst (σ : Term.Subst φ) (r : Block φ) : (r.vsubst σ).fl = r.fl := by simp
+
+@[simp]
+theorem BBRegion.fl_vsubst (σ : Term.Subst φ) (r : BBRegion φ) : (r.vsubst σ).fl = r.fl := by
+  induction r generalizing σ; simp [*]
+
+@[simp]
+theorem Region.fl_vsubst (σ : Term.Subst φ) (r : Region φ) : (r.vsubst σ).fl = r.fl := by
+  induction r generalizing σ <;> simp [*]
+
+-- TODO: Term.Subst.fv
+
+-- TODO: {Terminator, Region}.Subst.{fv, fl}
+
+-- TODO: fv_subst, fv_vsubst
+
+-- TODO: fl_lsubst
 
 end Subst
